AllStar/CorrectnessProof.v
@@ -1,4 +1,4 @@
-Require Import List String.
+Require Import List Omega String.
 Require Import Lib.Derivation Lib.Grammar Lib.Lemmas
                Lib.ParseTree Lib.Tactics Lib.Utils.
 Require Import AllStar.Parser AllStar.Subparser.
@@ -34,17 +34,243 @@ Proof.
       * inv H.
 Qed.
 
-Axiom silly_in_grammar : forall (g : grammar) x ys,
-    In (x, ys) g.
+(* Here are the lemmas we need to fill the gap in the proof below. *)
 
-(* Here's the lemma we need to fill the only hole in the proof below. *)
-Lemma startState_in_grammar : forall g x stack0 sps sp ys,
+Lemma beqSym_eq : forall x y,
+    beqSym x y = true <-> x = y.
+Proof.
+  intros; split; intros.
+  - unfold beqSym in H. destruct (SymbolMapFacts.eq_dec).
+    + subst; reflexivity.
+    + inv H.
+  - unfold beqSym. destruct (SymbolMapFacts.eq_dec).
+    + reflexivity.
+    + exfalso. apply n. assumption.
+Qed.
+
+(* Not needed anymore, since we proved this fact
+   about the version of rhss in Utils *)
+(*
+Lemma rhss_in_grammar : forall g ntName yss ys,
+    rhss g ntName = yss ->
+    In ys yss ->
+    In (NT ntName, ys) g.
+Proof.
+  intro g.
+  induction g as [| prod g']; intros ntName yss ys Hrhss Hin;
+  simpl.
+  - simpl in Hrhss. rewrite <- Hrhss in Hin. inv Hin.
+  - destruct prod as [l r]; subst. simpl in Hin.
+    destruct (beqSym l (NT ntName)) eqn:Heq.
+    + rewrite beqSym_eq in Heq. simpl in Hin.
+      destruct Hin as [Hhd | Htl].
+      * left. subst. reflexivity.
+      * right. eapply IHg'; [reflexivity | assumption].
+    + right. eapply IHg'; [reflexivity | assumption].
+Qed.
+*)
+
+Lemma spClosure_preserves_pred :
+  forall g freeSyms sp sps sp',
+    spClosure g freeSyms sp = sps ->
+    In sp' sps ->
+    sp.(pred) = sp'.(pred).
+Proof.
+  intros. unfold spClosure in H.
+  subst.
+  induction (gammaClosure g (freeSyms, stack sp))
+    as [| gamma gammas].
+  - simpl in H0. inv H0.
+  - destruct H0.
+    + subst. simpl. reflexivity.
+    + apply IHgammas. assumption.
+Qed.
+
+Lemma closure_preserves_preds :
+  forall g freeSyms sps sp' sps',
+    closure g freeSyms sps = sps' ->
+    In sp' sps' ->
+    exists sp,
+      In sp sps /\ sp.(pred) = sp'.(pred).
+Proof.
+  induction sps as [| sp sps]; intros.
+  - simpl in H. subst. inv H0.
+  - unfold closure in H.
+    subst. simpl in H0.
+    apply in_app_or in H0.
+    destruct H0.
+    + exists sp. split.
+      * apply in_eq.
+      * eapply spClosure_preserves_pred.
+        { reflexivity. }
+        { eassumption. }
+    + edestruct IHsps.
+      * reflexivity.
+      * unfold closure. eassumption.
+      * destruct H0.
+        exists x. split.
+        { apply in_cons. assumption. }
+        { assumption. }
+Qed.
+    
+Lemma startState_in_grammar :
+  forall g x stack0 sps sp gamma,
     startState g x stack0 = sps ->
-    In sp sps -> 
-    sp.(pred) = ys ->
+    In sp sps ->
+    sp.(pred) = gamma ->
+    In (NT x, gamma) g.
+Proof.
+  intros.
+  unfold startState in H.
+  eapply closure_preserves_preds in H.
+  - destruct H as [sp0]; destruct H.
+    rewrite in_map_iff in H.
+    destruct H as [gamma0]; destruct H.
+    subst. simpl in H2. subst.
+    eapply Utils.rhss_in_grammar.
+    + reflexivity.
+    + eassumption.
+  - assumption.
+Qed.
+
+Lemma nub_In :
+  forall A (x : A) xs xs' f,
+    nub xs f = xs' ->
+    In x xs' ->
+    In x xs.
+Proof.
+  induction xs as [| hd tl]; intros.
+  - simpl in H. subst. inv H0.
+  - simpl in H.
+    destruct (elem hd (nub tl f) f) eqn:Helem.
+    + apply IHtl in H.
+      * apply in_cons. assumption.
+      * assumption.
+    + subst. destruct H0.
+      * subst. apply in_eq.
+      * eapply IHtl in H.
+        { apply in_cons. assumption. }
+        { reflexivity. }
+Qed.
+
+Lemma move_preserves_preds :
+  forall token sps sp',
+    In sp' (move token sps) ->
+    exists sp,
+      In sp sps /\ sp.(pred) = sp'.(pred).
+Proof.
+  intros. unfold move in H.
+  induction sps as [| sp sps]; simpl in H.
+  - inv H.
+  - apply in_app_or in H. destruct H.
+    + destruct (stack sp).
+      * inv H.
+        { exists sp'; split.
+          { apply in_eq. }
+          { reflexivity. }}
+        { inv H0. }
+      * destruct s as [tName | ntName].
+        { destruct (beqSym (T tName) (T token)).
+          { inv H.
+            { exists sp; split.
+              { apply in_eq. }
+              { simpl. reflexivity. }}
+            { inv H0. }}
+          { inv H. }}
+        { inv H. }
+    + apply IHsps in H. clear IHsps.
+      destruct H as [sp'']; destruct H.
+      exists sp''; split.
+      * apply in_cons. assumption.
+      * assumption.
+Qed.
+    
+Lemma target_preserves_preds :
+  forall g sps token sp',
+    In sp' (target g sps token) ->
+    exists sp,
+      In sp sps /\ sp.(pred) = sp'.(pred).
+Proof.
+  intros. unfold target in H.
+  eapply closure_preserves_preds with
+      (sps := move token sps) in H.
+  -  destruct H as [sp]; destruct H.
+     apply move_preserves_preds in H.
+     destruct H as [sp0]; destruct H.
+     exists sp0; split.
+     + assumption.
+     + rewrite H1. assumption.
+  - reflexivity.
+Qed.
+  
+Lemma predict_preserves_preds :
+  forall g input ys sps,
+    predict g sps input = Choice ys ->
+    exists sp,
+      In sp sps /\ sp.(pred) = ys.
+Proof.
+  induction input as [| token tokens]; intros.
+  - unfold predict in H.
+    destruct (nub sps
+          (fun sp sp2 : subparser =>
+           beqList (pred sp) (pred sp2))) eqn:Hnub.
+    + inv H.
+    + destruct l.
+      * inv H.
+        exists s. split.
+        { eapply nub_In.
+          { reflexivity. }
+          { rewrite Hnub. apply in_eq. }}
+        { reflexivity. }
+      * destruct (conflict sps); inv H.
+  - unfold predict in H.
+    destruct (nub sps
+          (fun sp sp2 : subparser =>
+             beqList (pred sp) (pred sp2))) eqn:Hnub.
+    + inv H.
+    + destruct l.
+      * inv H.
+        exists s; split.
+        { eapply nub_In.
+          { reflexivity. }
+          {  rewrite Hnub. apply in_eq. }}
+        { reflexivity. }
+      * destruct (conflict sps).
+        { inv H. }
+        { unfold predict in IHtokens.
+          apply IHtokens in H. clear IHtokens.
+          destruct H as [sp']; destruct H.
+          apply target_preserves_preds in H.
+          subst. assumption. }
+Qed.
+            
+Lemma sllPredict_result_in_grammar :
+  forall g x input ys,
+    sllPredict g x input = Choice ys ->
     In (NT x, ys) g.
 Proof.
-Abort.
+  intros. unfold sllPredict in H.
+  apply predict_preserves_preds in H.
+  destruct H as [sp]; destruct H.
+  eapply startState_in_grammar in H.
+  - eassumption.
+  - reflexivity.
+  - assumption.
+Qed.
+
+Lemma llPredict_result_in_grammar :
+  forall g x input stack0 ys,
+    llPredict g x input stack0 = Choice ys ->
+    In (NT x, ys) g.
+Proof.
+  intros. unfold llPredict in H.
+  apply predict_preserves_preds in H.
+  destruct H as [sp]; destruct H.
+  eapply startState_in_grammar in H.
+  - eassumption.
+  - reflexivity.
+  - assumption.
+Qed.
 
 Lemma adaptivePredict_result_in_grammar :
   forall g x input stack0 ys,
@@ -53,10 +279,13 @@ Lemma adaptivePredict_result_in_grammar :
 Proof.
   intros. unfold adaptivePredict in H.
   destruct (sllPredict g x input) eqn:Hsll.
-  - inv H. 
-    unfold sllPredict in Hsll. unfold startState in Hsll.
-    unfold rhss in Hsll. simpl.
-Abort.
+  - inv H.
+    eapply sllPredict_result_in_grammar.
+    eassumption.
+  - eapply llPredict_result_in_grammar.
+    eassumption.
+  - inv H.
+Qed.
 
 Theorem parse'_correct :
   forall (g      : grammar)
@@ -127,10 +356,12 @@ Proof.
               { (* Here's where we need a lemma saying that
                    whenever adaptivePredict returns Choice ys,
                    ys is in the grammar. *)
-                apply silly_in_grammar. }
+                eapply adaptivePredict_result_in_grammar.
+                eassumption. }
               apply derivesFnil. }
             eapply derivesNT.
-            { apply silly_in_grammar. }
+            { eapply adaptivePredict_result_in_grammar.
+              eassumption. }
             eapply derivesFcons.
             { eassumption. }
             eassumption. }
@@ -199,4 +430,3 @@ Theorem parse_correct :
 Proof.
   intros. eapply parse'_correct. eassumption.
 Qed.
-
